### $$if\ h(x) = \frac{f(x)}{g(x)}$$
### $$\downarrow$$
### $$ h'(x) = \frac{g(x)f'(x) - f(x)g'(x)}{[g(x)]^2}$$
_______

### $$ \frac{dy}{dx} = \frac{v\frac{du}{dx} - u\frac{dv}{dx}}{v^2}$$
______
### $$d(\frac{u}{v}) = \frac{du*v - dv*u}{v^2}$$
_______
### Proof
$$q(x) = \frac{f(x)}{g(x)} = f(x) * (g(x))^{-1}$$
$$using\ the\ product\ law$$
$$q'(x) = f'(x) * (g(x))^{-1} + Dx[(g(x))^{-1}]*f(x)$$
$$Dx[(g(x))^{-1}]\ use\ chain\ rule\ \downarrow$$
$$= -1(g(x))^{-2} * g'(x)$$
$$\therefore q'(x) = \frac{f'(x)}{g(x)} + \frac{f(x) * -g'(x)}{g(x)^2}$$
$$ = \frac{f'(x)g(x) - f(x)g'(x)}{g(x)^2}$$
_____
### Example
