$$ y = \frac{2}{\sqrt{3x+1}}$$
$$ y = 2(3x+1)^{-\frac12}$$
$$ let = 3x+1 = u$$
$$y = 2u^{-\frac12}$$

$$\frac{dy}{du} = -1u^{-\frac32}$$
$$\frac{du}{dx} = 3$$
$$\frac{dy}{dx} = \frac{dy}{du} * \frac{du}{dx}$$
$$ = -1u^{-\frac32}(3) = -3u^{-\frac32}$$
$$ = -3(3x+1)^{-\frac32}$$


$$\begin{align}\
\\
\\
\\
\end{align}$$
$$f(x) = \frac{3}{x^2+4x-2}$$
$$ = 3(x^2+4x-2)^{-1}$$
$$x^2 + 4x - 2 = u$$
$$ y = 3u^{-2}$$
$$\frac{dy}{du} = -3u^{-2}$$
$$\frac{du}{dx} = 2x + 4$$
$$\frac{dy}{dx} = \frac{dy}{du} * \frac{du}{dx}$$
$$= -3u^{-2} (2x+4)$$
$$= \frac{-3(2x+4)}{(x^2+4x-2)^2}$$

#### Simpler way:

differentiate the outer function and then the inner function and then multiply them together.

$$ f'(x) = -3(x^2+4x-2)^{-2}*(2x+4)$$

### Important!
The number on the outside of the bracket is a constant. If it contains a variable then you must use [[Product Rule]].