### Example
Convert the following to polar form
1. $z = -2(\cos\alpha+i\sin\alpha)$
2. $z = -2(\cos\alpha - i\sin\alpha)$
3. $z = 2(\cos\alpha-i\sin\alpha)$


1.  
   $$z = 2(-\cos\alpha - i \sin\alpha)$$
   $$third\ quadrant$$
   $$\downarrow$$
   $$= 2(\cos(\alpha-\pi) + \sin(\alpha-\pi))$$

2. 
$$z = 2(-\cos\alpha + i\sin\alpha) $$
$$=2(\cos(\pi-\alpha) + i\sin(\pi-\alpha))$$

3. 
   $$z=2(\cos(-\alpha) + i\sin(-\alpha))$$

##### Always:
- Use algebra if possible
- Sketch graph to see roots easier
- Always state the degree of accuracy