- [[Waves]]

![[Pasted image 20230725134756.png]]

## $$Eg\ Sin30^o = \frac{y}{r} = \frac12$$
## Reductions

$$sin110^o = sin70^o$$
$$sin285^o = -sin75^o$$
$$sin-40^o = -sin40^o$$
$$sin200^o = -sin20^o$$
$$sin360^o-\theta = -sin\theta$$
$$sin180^o+\theta = -sin\theta$$
$$sin180^o-\theta = sin\theta$$
$$\begin{align}\
\\
\\
\end{align}$$
$$sin\frac{5\pi}{4} = -sin\frac{\pi}{4} $$
$$cos3\pi = cos\pi$$
$$tan\frac{7\pi}8 = -tan\frac{\pi}8$$
$$sin \frac{5\pi}6 = sin\frac{\pi}6$$

## $$sin(90^o-\theta) = cos\theta$$
![[Pasted image 20230725140030.png]]

![[Pasted image 20230823171109.png]]

### _Special Angles: 30, 60, 45, 0, 180, 90_

### $$tan45^o = \frac{\sqrt2}{\sqrt2} = 1$$
### $$ sin45^o=\frac{o}h = \frac{\sqrt2}2 = \frac1{\sqrt2}$$
# $$ tan\theta = \frac{sin\theta}{cos\theta} $$
# $$ sin^2\theta + cos^2\theta = 1$$
# $$ \therefore cos^2\theta = 1-sin^2\theta $$
# $$ \therefore sin^2\theta = 1-cos^2\theta$$


### <u>Example</u>
The obtuse angle x radians is such that tanx = -k
where k is a positive constant and π/2 <= x <= π

$$tan\theta = \frac{k}{-1} = \frac{y}x$$
$$tan\theta = -k = \frac{-k}1 = \frac{k}{-1}$$
a)
$$ tan-x = \frac{-k}{1} = k $$
$$ \therefore\ opposite = k$$
$$ adjacent = -1$$
$$hypotenuse = \sqrt{k^2+1}$$




## Trig Graphs

### $$ y = a*sin(bx-c) + d$$
$$ a - Vertical\ Stretch\ SF * a $$
$$ -a - Reflection$$
$$b - Horizontal\ Stretch$$
$$c - Horizontal\ Translation $$
$$d - Vertical\ Translation$$

![[Pasted image 20230725185627.png]]
![[Pasted image 20230725185641.png]]


### Domain:

### $$x \epsilon [-x^o, y^o] $$

### $$ -x^o \le x \le y^o x \epsilon R $$

### Stretches and Translations:

Order of the 2 matters !!!

$$ y = 3sinx + 4$$
(1) Stretch
(2) Translate

SF x3
Translation - Up 4

$$ y = 2 cos(3x - 60^o)$$
$$ (1)\ Vertical\ stretch\ SF x2$$
$$(2)\ Period\ x3$$
$$(3)\ Translation - Right\ 60$$

## $$ Tp = \frac{90^o}{b}$$
## $$Period = \frac{360^o}{b}$$
## Inverse Trig

![[Pasted image 20230725200800.png]]



## Trig Equations

### <u>Examples:</u>

$$ (\frac{1}{sinx} - sinx)^2 = \frac1{tan^2x} - cos^2x$$
$$LHS\ \ \ \ \ \ \ \ \ \ \ \ \ \ \ \ \ \ \ \ \ RHS$$
$$RHS = \frac{cos^2x}{sin^2x} - \frac{cos^2x}1$$
$$ = \frac{cos^2x - sin^2x*cos^2x}{sin^2x}$$
$$ =\frac{cos^2x*cos^2x}{sin^2x} = \frac{cos^4x}{sin^2x}$$
$$\begin{align}\
\\
\end{align}$$
$$ LHS = (\frac{1-sin^2x}{sinx})^2$$
$$ = \frac{cos^2x}{sinx}$$
$$ = \frac{cos^4x}{sin^2x} = RHS$$
______
### <u>General Solutions:</u>

<u>Sine</u>
$$x = \theta + k*360^o$$
$$ x = \theta + k*2\pi$$
$$\begin{align}\
\\
\\
\end{align}$$
$$ x = (180^o - \theta) + k*360^o$$
$$ x = (\pi - \theta) + k*2\pi$$
$$k \epsilon Z$$


<u>Cosine</u>
$$ x = \theta + k*360$$
$$ x = -\theta +k*360$$
$$\begin{align}\
\\
\end{align}$$
$$ x = \theta + k*2\pi$$
$$ x = -\theta + k*2\pi$$


<u>Tangent</u>
$$ x= \theta + k*180^o$$
$$ x = \theta + k*\pi$$
______
## Types of Trig. equations

### Type 1 - Simple

$$cos3\theta = -0.5$$
$$\theta \epsilon [-90^o, 120^o]$$
$$\begin{align}\
\\
\\
\end{align}$$
$$3\theta = 120^o + k*360^o$$
$$\theta = 40^o + k*120^o$$
$$ k \epsilon Z$$
$$ 3\theta = -120^o + k*360^o$$
$$\theta = -40^o + k*120^o$$
$$\theta \epsilon [-40^o,40^o,-80^o,80^o]$$



### Type 2 - Horizontal Translation
$$ cos2\theta = cos(\theta + 40^o)$$
$$ \theta \epsilon [-180^o, 180^o]$$
$$\begin{align}\
\\
\\
\end{align}$$
$$2\theta = \theta + 40^o + k*360^o$$
$$2\theta = -(\theta + 40^o) + k*360^o$$
$$k \epsilon Z$$
$$\theta = 40^o + k*360^o$$
$$\theta = -13.3^o + k*120^o$$
$$ \theta \epsilon [40^o, -13.3^o, 100.7^o]$$



### Type 3 - Reductions
$$ sin2\theta = -sin\theta$$
$$\theta \epsilon [-\pi, \pi]$$
$$\begin{align}\
\\
\\
\end{align}$$
$$ sin2\theta = sin-\theta$$
$$2\theta = -\theta +k*2\pi$$
$$2\theta = (\pi-(-\theta)) + k*2\pi$$
$$\frac{3\theta}{3} = \frac{k*2\pi}{3}$$
$$\theta = k*2\pi$$
$$\theta \epsilon [\frac{2\pi}3, \frac{-2\pi}3, \pi, -\pi]$$



### Type 4 - Change of Ratio
$$ cos(\theta + 60^o) = sin2\theta$$
$$ \theta \epsilon [-180^o, 180^o]$$
$$\begin{align}\
\\
\\
\end{align}$$
$$cos(\theta + 60^o) = cos(90^o - 2\theta)$$
$$\theta + 60^o = 90^o - 2\theta+k*360^o$$
$$\theta + 60^o = -(90^o-2\theta) + k*360^o$$
$$ 3\theta = 90^o -60^o + k*360$$
$$\theta = 10^o = k*120^o$$
$$\theta + 60^o = -90^o + 2\theta + k*360^o$$
$$ -\theta = -150^o + k*360^o$$
$$\theta = 150^o + k*360^o$$
