### $$ y = ax^2 + bx + c$$
### $$y = a(x - b)(x - c) $$
### $$ y = a(x-p)^2 + q$$


![[Pasted image 20230805141125.png]]

![[Pasted image 20230805141223.png]]
When a = 1 or -1 the graph can be sketched from the turning point by going:

- out 1 up 1
- out 2 up 4
- out 3 up 9

_note that the y-value graphed is is x value squared_

### Transformations
$$ y = a(x-p)^2 + q$$
$p$ - left/right transformation (inverted)
$q$ - up/down transformation


#### <mark class="hltr-blue">Vertical</mark>

$f(x) = x^2 - 2x+1$

$\begin{bmatrix} 0 \\ 4 \\ \end{bmatrix}$

$f(x) + 4 = (x^2 -2x + 1) + 4$

$= x^2 -2x + 5$


$g(x) = 3(x-5)^2 + 1$

$g(x) + 4 = 3(x-5)^2 + 1 + 4$

$= 3(x-5)^2 + 5$


### <mark class="hltr-cyan">Horizontal</mark>

$f(x) = x^2-2x+1$

$f(x + 3) = (x+3)^2 - 2(x+3)+1$

$f(x+3)$ - Backwards / will move graph 3 left

$= x^2 + 6x + 9 - 2x-6+1$

$= x^2 + 4x + 4$
