### $$e = 2.7182818...$$
### $$y = e^x$$
### $$\ln_ey = x$$
### $$\ln e = 1$$
### Fun Facts
If you compound an investment of $\$1$, with an interest rate of 100% an infinite number of times, the annual return tends to be e.
$$ A = p(1 + \frac{r}n)^{nt}$$
$$A = 1(1+\frac1n)^n$$
$$A = \lim_{n \rightarrow \infty}\ (1 + \frac1n)^n$$
$$= 2.7182... = e$$

______
### Examples
1) $$\ln e^5$$
$$=5\ln e$$
$$ = 5$$
2) $$\ln 0$$
$$= no\ sol.\ /\ -\infty$$
3) $$\ln e^{-3} + \ln e^12$$
$$-3\ln e + 12 \ln e$$
$$ = -3 + 12$$
$$= 9$$
4) $$\ln (\frac{1}{e^{24}})$$
$$ = \ln e^{-24}$$
$$= -24 \ln e = -24$$
5) $$ \frac{(\ln e ^2)^6}{(\ln e^3)^4}$$
$$=\frac{(2\ln e)^6}{(3\ln e)^4}$$
$$= \frac{2^6}{3^4}$$
$$= \frac{64}{81}$$
6) $$ 1-2\ln x = -4$$
$$ -2 \ln x = -5$$
$$ \ln x = \frac52$$
$$e^{\frac52} = x$$
7) $$Make\ p\ the\ subject\ of\ \ln p - \ln 1-p = t$$
$$\ln p -\ln (1-p) = t$$
$$\ln \frac{p}{1-p} = t$$
$$e^t = \frac{p}{1-p}$$
$$e^t(1-p) = p$$
$$e^t - e^tp = p$$
$$e^t = p + e^tp$$
$$\frac{e^t}{1+e^t} = \frac{p(1+e^t)}{1+e^t}$$
$$p = \frac{e^t}{1+e^t}$$
8) $$e^{2x} + e^x = 6$$
$$e^x = k$$
$$k^2 + k - 6 = 0$$
$$(k+3)(k-2) = 0$$
$$e^x = -3$$
$$No\ Sol.$$
$$e^x = 2$$
$$\ln 2 = x$$
$$x = 0.693$$
______
