### $$\frac{px + q}{(ax + b)(cx + d)(ex + f)} \equiv \frac{A}{(ax + b)} + \frac{B}{(cx + d)} + \frac{C}{(ex + f)}$$
### $$\frac{px^2 + qx + r}{(ax + b)(cx^2 + d)} \equiv \frac{A}{(ax + b)} + \frac{Bx + C}{(cx^2 + d)}$$
### $$\frac{px^2 + qx + r}{(ax + b)(cx + d)^2} \equiv \frac{A}{(ax + b)} + \frac{B}{(cx + d)} + \frac{C}{(cx + d)^2}$$
### $$\frac{px^2 + qx + r}{(ax-b)(cx - d)} \equiv A + \frac{B}{(ax+b)} + \frac{C}{cx + d} $$
____
### Example
Express $\frac{4 + x}{(1 + x)(2 - x)}$ as a sum of partial fractions.
$$\frac{4 +x}{(1 + x)(2 -x)} = \frac{A}{(1 + x)} + \frac{B}{(2-x)}$$
Multiply both sides by $(1 + x)(2-x)$.
$$4 + x = A(2-x) + B(1 + x)$$
Substitute in the only value of x that will make one of the brackets = 0.
$$x = -1$$
$$4 + x = A(2-x)$$
$$4 + (-1) = A(2 -(-1))$$
$$3 = 3A$$
$$A = 1$$
$$\downarrow$$
$$x = 2$$
$$4 + (2) = B(1 + (2))$$
$$6 = 3B$$
$$B = 2$$
$$\therefore\  = \frac{1}{1 + x} + \frac{2}{2-x}$$

Or do simultaneous equations if you cannot make the brackets cancel.
_____
Express $\frac{4x^3 + 10x + 4}{x(2x + 1)}$ in partial fractions.

$$2x^2 + x \ \ \overline{)4x^3 + 10x + 4}$$
$$= 2x - 1$$
$$r = 11x + 4$$
$$\downarrow$$
$$2x -1 + \frac{11x + 4}{2x^2 + x}$$

$$\frac{11x + 4}{x(2x + 1)} = \frac{A}{x} + \frac{B}{(2x + 1)}$$
$$11x + 4 = A(2x +1) + B(x)$$
$$\downarrow$$
$$x = 0 $$
$$A = 4$$
$$\downarrow$$
$$x = -\frac12$$
$$B = 3$$
$$\downarrow$$
$$= 2x -1 + \frac4x + \frac{3}{2x + 1}$$
________
Express $\frac4{(1-3x)(1-x)^2}$ as a sum of partial fractions.
$$= \frac{A}{(1-3x)} + \frac{B}{(1-x)} + \frac{C}{(1-x)^2}$$
$$4 = A(1-x)^2 + B(1-3x)(1-x)^2 + C(1-3x)$$
$$when\ x=1\ \rightarrow C = -2$$
$$when\ x=\frac13 \rightarrow A = 9$$
$$Equate\ the\ coefficients\ of\ x^0$$
$$4 = A + B + C$$
$$B =  -3$$
$$\downarrow$$
$$= \frac{9}{1-3x} - \frac{3}{1-x} - \frac{2}{(1-x)^2}$$
