### $$ \sin(2A) = 2\sin(A)\cos(A)$$
### $$\cos(2A) = 1 - 2\sin^2(A)$$
### $$\cos(2A) = 2\cos^2(A) - 1$$
### $$\cos(2A) = \cos^2(A) - \sin^2(A)$$
### $$\tan(2A) = \frac{2\tan(A)}{1-\tan^2(A)}$$
_______

### Proofs
1) $$\sin2A = \sin(A + A)$$
$$= \sin A\cos A + \sin A \cos A$$
$$= 2\sin A \cos A$$

2) $$ \cos 2A = \cos(A + A)$$
$$\cos A \cos A + \sin A \sin A$$
$$\cos^2A - \sin^2A$$

3) $$(1-\sin^2A) - \sin^2 A$$
$$1 - 2\sin^2A$$
4) $$\cos 2A = \cos^2 A - (1 - \cos^2 A)$$
$$ = 2\cos^2A - 1$$

5) $$\tan 2A = \tan(A + A)$$
$$ = \frac{\tan A + \tan A}{1 - \tan A \tan A}$$
$$ = \frac{2\tan A}{1 - \tan^2 A}$$
______
### Example
WS #2, Q7

$$\frac{1 - \sin2x}{\sin x - \cos x}$$
$$=\frac{1 - 2\sin x \cos x}{\sin x - \cos x}$$
$$ = \frac{\cos^2x + \sin^2x - 2\sin x \cos x}{\sin x - \cos x}$$
$$ = \frac{(\cos x - \sin x)(\cos x - \sin x)}{\sin x - \cos x}$$
$$ = \frac{-(\sin x - \cos x) (\cos x - \sin x)}{(\sin x - \cos x)}$$
$$ = -\cos x + \sin x \rightarrow \sin x - \cos x$$
$$\therefore LHS\ =\ RHS$$
